src/theory/QueryAuxLemmas.v
@@ -65,15 +65,15 @@ Section Theory.
   
   Transparent oqresponse_name qresponse_name is_field.
 
-  Variables Vals : eqType.
+  Variables Value : eqType.
 
-  Implicit Type φ : seq (@Selection Vals).
-  Implicit Type selection : @Selection Vals.
+  Implicit Type φ : seq (@Selection Value).
+  Implicit Type selection : @Selection Value.
 
   (** ---- *)
   (** *** Other types of predicates *)
   Section DefPreds.
-    Variable (s : @wfGraphQLSchema Vals).
+    Variable (s : @wfGraphQLSchema Value).
 
     
     (** ---- *)
@@ -145,7 +145,7 @@ Section Theory.
     (**
        This lemma states that if the size of queries is 0, that means the list is empty.
      *)
-    Lemma queries_size_0_nil (qs : seq (@Selection Vals)) : queries_size qs == 0 -> qs = [::].
+    Lemma queries_size_0_nil (qs : seq (@Selection Value)) : queries_size qs == 0 -> qs = [::].
     Proof.
         by case: qs => //=; case.
     Qed.
@@ -155,12 +155,12 @@ Section Theory.
     (**
        This lemma states that if the size of queries is 0, that means the list is empty.
      *)
-    Lemma queries_size_aux_0_nil (nq : seq (Name * @Selection Vals)) : queries_size_aux nq == 0 -> nq = [::].
+    Lemma queries_size_aux_0_nil (nq : seq (Name * @Selection Value)) : queries_size_aux nq == 0 -> nq = [::].
     Proof.
         by case: nq => //=; case=> ty; case.
     Qed.
 
-    Lemma queries_size_aux_cat (σs1 σs2 : seq (Name * @Selection Vals)) : 
+    Lemma queries_size_aux_cat (σs1 σs2 : seq (Name * @Selection Value)) : 
       queries_size_aux (σs1 ++ σs2) = queries_size_aux σs1 + queries_size_aux σs2.
     Proof.
       case: σs1 σs2 => //= σ σs1 σs2.
@@ -168,7 +168,7 @@ Section Theory.
       
     Qed.
     
-    Lemma queries_size_aux_tr (σs : seq (@Selection Vals)) t n :
+    Lemma queries_size_aux_tr (σs : seq (@Selection Value)) t n :
       queries_size σs <= n ->
       queries_size_aux [seq (t, σ) | σ <- σs] <= n.
     Proof.
@@ -185,7 +185,7 @@ Section Theory.
      Lemmas about functions used to find queries 
    *)
   Section Find.
-    Variable (s : @wfGraphQLSchema Vals).
+    Variable (s : @wfGraphQLSchema Value).
 
     (** ---- *)
     (**
@@ -218,7 +218,7 @@ Section Theory.
     (**
        This lemma states that that [find_queries_with_label] distributes over list concatenation.
      *)
-    Lemma find_queries_with_label_cat l ty (qs1 qs2 : seq (@Selection Vals)):
+    Lemma find_queries_with_label_cat l ty (qs1 qs2 : seq (@Selection Value)):
       find_queries_with_label s l ty (qs1 ++ qs2) = find_queries_with_label s l ty qs1 ++ find_queries_with_label s l ty qs2.
     Proof.
       funelim (find_queries_with_label s l ty qs1) => //=.
@@ -238,7 +238,7 @@ Section Theory.
         by rewrite queries_size_cat; ssromega.
     Qed.
 
-    Lemma found_pairs_with_response_name_leq rname (σ : seq (Name * @Selection Vals)) :
+    Lemma found_pairs_with_response_name_leq rname (σ : seq (Name * @Selection Value)) :
       queries_size_aux (find_pairs_with_response_name rname σ) <= queries_size_aux σ.
     Proof.
       rewrite /queries_size_aux.
@@ -251,7 +251,7 @@ Section Theory.
     (**
        This lemma states that
      *)
-    Lemma find_map_inline_nil_func (f : Name -> seq (@Selection Vals) -> seq Selection) rname t ptys φ :
+    Lemma find_map_inline_nil_func (f : Name -> seq (@Selection Value) -> seq Selection) rname t ptys φ :
       uniq ptys ->
       all (is_object_type s) ptys ->
       t \notin ptys ->
@@ -375,7 +375,7 @@ Section Theory.
        with [find_pairs_with_response_name] is the same as first projecting the second element 
        and then applying [find_fields_with_response_name].
      *)
-    Lemma find_pairs_spec rname (nq : seq (Name * @Selection Vals)) :
+    Lemma find_pairs_spec rname (nq : seq (Name * @Selection Value)) :
       [seq q.2 | q <- find_pairs_with_response_name rname nq] = find_fields_with_response_name rname [seq q.2 | q <- nq].
     Proof.
       move: {2}(queries_size_aux _) (leqnn (queries_size_aux nq)) => n.
@@ -397,7 +397,7 @@ Section Theory.
        fragments with a type condition that was not in the original list of type conditions
        results in a empty list.
      *)
-    Lemma find_fragment_inlined_nil_func t ptys (f : Name -> seq (@Selection Vals) -> seq (@Selection Vals)) φ :
+    Lemma find_fragment_inlined_nil_func t ptys (f : Name -> seq (@Selection Value) -> seq (@Selection Value)) φ :
       t \notin ptys ->
       find_fragment_with_type_condition t [seq InlineFragment t' (f t' φ) | t' <- ptys] = [::].
     Proof.
@@ -441,7 +441,7 @@ Section Theory.
     (**
        This lemma states that
      *)
-    Lemma filter_pairs_spec rname (nq : seq (Name * @Selection Vals)) :
+    Lemma filter_pairs_spec rname (nq : seq (Name * @Selection Value)) :
       [seq q.2 | q <- filter_pairs_with_response_name rname nq] = filter_queries_with_label rname [seq q.2 | q <- nq].
     Proof.
       elim: nq => //= q nq IH.
@@ -463,7 +463,7 @@ Section Theory.
     Qed.
 
 
-    Lemma filter_pairs_with_response_name_leq rname (σ : seq (Name * @Selection Vals)) :
+    Lemma filter_pairs_with_response_name_leq rname (σ : seq (Name * @Selection Value)) :
       queries_size_aux (filter_pairs_with_response_name rname σ) <= queries_size_aux σ.
     Proof.
       rewrite /queries_size_aux.
@@ -476,7 +476,7 @@ Section Theory.
     (**
        This lemma states that [filter_queries_with_label] distributes over list concatenation.
      *)
-    Lemma filter_queries_with_label_cat l (qs1 qs2 : seq (@Selection Vals)) :
+    Lemma filter_queries_with_label_cat l (qs1 qs2 : seq (@Selection Value)) :
       filter_queries_with_label l (qs1 ++ qs2) = filter_queries_with_label l qs1 ++ filter_queries_with_label l qs2.
     Proof.
       elim: qs1  => //= hd tl IH.
@@ -489,7 +489,7 @@ Section Theory.
     (**
        This lemma states that the order of filtering with two response names does not affect the result.
      *)
-    Lemma filter_swap rname1 rname2 (φ : seq (@Selection Vals)) :
+    Lemma filter_swap rname1 rname2 (φ : seq (@Selection Value)) :
       filter_queries_with_label rname1 (filter_queries_with_label rname2 φ) =
       filter_queries_with_label rname2 (filter_queries_with_label rname1 φ).
     Proof.
@@ -503,7 +503,7 @@ Section Theory.
        This lemma states that filtering twice with the same response name is the same 
        as filtering once.
      *)
-    Lemma filter_filter_absorb rname (φ : seq (@Selection Vals)) :
+    Lemma filter_filter_absorb rname (φ : seq (@Selection Value)) :
       filter_queries_with_label rname (filter_queries_with_label rname φ) = filter_queries_with_label rname φ.
     Proof.
       funelim (filter_queries_with_label rname φ) => //=; simp filter_queries_with_label; do ? by rewrite Heq /= H.
@@ -515,9 +515,9 @@ Section Theory.
     (**
        This lemma states that
      *)
-    Lemma filter_map_inline_func (f : Name -> seq (@Selection Vals) -> seq Selection) rname φ ptys :
+    Lemma filter_map_inline_func (f : Name -> seq (@Selection Value) -> seq Selection) rname φ ptys :
       filter_queries_with_label rname [seq InlineFragment t (f t φ) | t <- ptys] =
-      [seq @InlineFragment Vals t (filter_queries_with_label rname (f t φ)) | t <- ptys].
+      [seq @InlineFragment Value t (filter_queries_with_label rname (f t φ)) | t <- ptys].
     Proof.
         by elim: ptys => //= t ptys IH; simp filter_queries_with_label; rewrite IH.
     Qed.
@@ -568,7 +568,7 @@ Section Theory.
     Qed.
 
     
-    Variable (s : @wfGraphQLSchema Vals).
+    Variable (s : @wfGraphQLSchema Value).
 
     
     (** ---- *)
@@ -640,7 +640,7 @@ Section Theory.
     (**
        This lemma states that [merge_selection_sets] distributes over list concatenation.
      *)
-    Lemma merge_selection_sets_cat (qs1 qs2 : seq (@Selection Vals)) :
+    Lemma merge_selection_sets_cat (qs1 qs2 : seq (@Selection Value)) :
       merge_selection_sets (qs1 ++ qs2) = merge_selection_sets qs1 ++ merge_selection_sets qs2.
     Proof.
         by rewrite /merge_selection_sets map_cat flatten_cat.
@@ -660,7 +660,7 @@ Section Theory.
     Qed.
 
 
-    Variable (s : @wfGraphQLSchema Vals).
+    Variable (s : @wfGraphQLSchema Value).
 
 
     (** ---- *)
@@ -668,7 +668,7 @@ Section Theory.
        This lemma states that the size of queries obtained via [merge_pairs_selection_sets]
        is less or equal than the size of the original list of queries.
      *)
-    Lemma merge_pair_selections_leq (nq : seq (Name * @Selection Vals)) :
+    Lemma merge_pair_selections_leq (nq : seq (Name * @Selection Value)) :
       queries_size_aux (merge_pairs_selection_sets s nq) <= queries_size_aux nq.
     Proof.
       rewrite /queries_size_aux; funelim (merge_pairs_selection_sets s nq) => //=; simp selection_size; do ? ssromega;
